the `slim_check` tactic now uses the type class `testable` to build counterexamples

test/slim_check/examples.lean
@@ -22,4 +22,27 @@ by expect_failure { slim_check }
 example : 1 < (2 : ℕ) :=
 by slim_check
 
+def even (n : ℕ) : bool :=
+n % 2 = 0
+
+example : (∀ (α : Type) (xs : list α), xs.length < 10) :=
+by expect_failure { slim_check }
+
+example : (∀ (α : Type) (xs : list α), xs.length < 10) :=
+by expect_failure { slim_check }
+
+example : (∀ n m : ℕ, 2*m + n < 100) :=
+by expect_failure { slim_check }
+
+example : (∀ (n : ℤ) (xs : list ℤ) x, x ∈ xs → x < n) :=
+by expect_failure { slim_check }
+
+example : (∀ n m : ℕ, even m → ¬ even n → ¬ even (m+n)) :=
+by slim_check
+
+variables n m : ℕ
+
+example : (even m → ¬ even n → ¬ even (m+n)) :=
+by slim_check
+
 end slim_check.examples
