test/slim_check/tactics.lean
@@ -2,19 +2,34 @@
 import ...test.slim_check.testable
 
 namespace tactic.interactive
-open tactic
+open tactic slim_check
+
+meta def revert_all : tactic unit := do
+xs ← local_context,
+match xs with
+ | (x :: xs) := tactic.revert x >> revert_all
+ | [] := return ()
+end
 
 meta def slim_check : tactic unit := do
+revert_all,
 t ← target,
 p ← is_prop t,
 when (¬ p) (fail "expecting a proposition"),
-`[apply of_as_true, trivial]
+t' ← eval_expr Prop t,
+e ← to_expr ``(testable.run %%t),
+run ← eval_expr (gen test_result) e,
+let hinst : testable t' := ⟨ _, run ⟩,
+r ← run_io (@testable.check t' hinst),
+if r then admit else fail "found counter examples"
 
-meta def expect_failure (cmd : itactic) : tactic unit := do
-x ← try_core cmd,
-match x with
- | (some x) := fail "tactic is expected to fail"
- | none := admit
+open interaction_monad.result.
+
+meta def expect_failure (cmd : itactic) : tactic unit :=
+λ s, match cmd s with
+| (interaction_monad.result.exception _ _ s') := (trace s' >> admit) s
+| (interaction_monad.result.success a s) :=
+   mk_exception "success_if_fail combinator failed, given tactic succeeded" none s
 end
 
 end tactic.interactive
