test/slim_check/testable.lean
@@ -9,17 +9,38 @@ variable f : Type → Sort v
 
 namespace slim_check
 
+inductive test_result
+| success
+| gave_up : ℕ → test_result
+| failure : (list string) → test_result
+
 class testable (α : Sort u) :=
-  (run : gen (option (list string)))
+  (run : gen test_result)
 
 open list
+
+
+open test_result
+
+instance imp_dec_testable (p : Prop) [decidable p] (β : p → Sort u)
+  [∀ h, testable (β h)]
+: testable (Π h, β h) :=
+⟨ _,
+  do
+    if h : p
+    then testable.run (β h)
+    else return $ gave_up 1 ⟩
+
+def add_to_counter_example (x : string) : test_result → test_result
+ | (failure xs) := failure $ x :: xs
+ | x := x
 
 instance all_types_testable [testable (f ℤ)]
 : testable (Π x, f x) :=
 ⟨ (Π x, f x),
   do
     r ← testable.run (f ℤ),
-    return $ (cons $ "ℤ") <$> r ⟩
+    return $ add_to_counter_example "ℤ" r ⟩
 
 instance pi_testable [has_to_string α] [arbitrary α] [∀ x, testable (β x)]
 : testable (Π x : α, β x) :=
@@ -28,10 +49,10 @@ instance pi_testable [has_to_string α] [arbitrary α] [∀ x, testable (β x)]
   x ← arby α,
   gen.up (do
     r ← testable.run (β x),
-    return $ (cons $ to_string x) <$> r) ⟩
+    return $ add_to_counter_example (to_string x) r) ⟩
 
 instance de_testable {p : Prop} [decidable p] : testable p :=
-⟨ p, return $ if p then none else some [] ⟩
+⟨ p, return $ if p then success else failure [] ⟩
 
 section io
 
@@ -42,25 +63,46 @@ variable [io.interface]
 
 open nat
 
-def testable.run_suite_aux : ℕ → rand (option (list string))
- | 0 := return none
+def retry (cmd : rand test_result) : ℕ → rand test_result
+ | 0 := return $ gave_up 1
  | (succ n) := do
-x ← testable.run α' (99 - n),
-option.rec_on x (testable.run_suite_aux n) (return ∘ some)
+r ← cmd,
+match r with
+ | success := return success
+ | (failure xs) := return (failure xs)
+ | (gave_up _) := retry n
+end
+
+def give_up_once (x : ℕ) : test_result → test_result
+ | success := gave_up x
+ | (gave_up n) := gave_up (n+x)
+ | (failure xs) := failure xs
+
+def testable.run_suite_aux : test_result → ℕ → rand test_result
+ | r 0 := return r
+ | r (succ n) := do
+x ← retry (testable.run α' (99 - n)) 10,
+match x with
+ | success := testable.run_suite_aux r n
+ | (failure xs) := return (failure xs)
+ | (gave_up g) := testable.run_suite_aux (give_up_once g r) n
+end
 
 def testable.run_suite :=
-testable.run_suite_aux α' 100
+testable.run_suite_aux α' success 100
 
-def testable.check : io unit := do
+def testable.check : io bool := do
 x ← io.run_rand (testable.run_suite α'),
 match x with
- | none := io.put_str_ln "Success!"
- | (some xs) := do
+ | success := io.put_str_ln "Success!" >> return tt
+ | (gave_up n) := io.put_str_ln ("Gave up " ++ repr n ++ " times") >> return tt
+ | (failure xs) := do
    io.put_str_ln "\n===================",
    io.put_str_ln "Found problems!",
    io.put_str_ln "",
    list.mmap' io.put_str_ln xs,
-   io.put_str_ln "-------------------"
+   io.put_str_ln "-------------------",
+   return ff
 end
 
 end io
